Generalize And-I to arbitrary terms
This replaces And-I by:

    Γ ⊢ t: T     Γ ⊢ t: U
    ----------------------(And-I')
        Γ ⊢ t: T ∧ U

This required generalizing the type_safety theorem, the previous theorem was
stated in the paper as:

 ∀ρ,t,T. if (ρ ∅ ⊢ t : T), then
   either ∃y.  t = y and ρ(y) = {d}
   or ∃ρ1,t1.  (ρ t → t1 ρ1) and (ρ1 ∅ ⊢ t1 : T)

Notice that the preservation statement is weaker than usual here: it states that
there is a specific `t1` that `t` can step to which preserves the type, we can
generalize it to:

 ∀ρ,t,T. if (ρ ∅ ⊢ t : T), then we have both:
   - either ∃y. t = y and ρ(y) = {d}
     or ∃ρ1,t1. (ρ t → t1 ρ1)
   - and  ∀ρ2,t2. (ρ t → t2 ρ2) implies (ρ2 ∅ ⊢ t2 : T)

This gives us a stronger induction hypothesis which is key to the And-I' subcase
where t is not a value: by the IH, we obtain `Γ ⊢ t2: T` and `Γ ⊢ t2: U` for
some `t2` whereas previously we could only get `Γ ⊢ t2: T` and `Γ ⊢ t3: U` for
some `t2,t3` and therefore couldn't use (And-I') to complete the case.

oopsla16/dot.v
@@ -258,10 +258,10 @@ Inductive has_type : tenv -> venv -> tm -> ty -> nat -> Prop :=
       has_type GH G1 t T1 n1 ->
       stp GH G1 T1 T2 n2 ->
       has_type GH G1 t T2 (S (n1 + n2))
-  | T_AndI : forall GH G1 b x T1 T2 n1 n2,
-      has_type GH G1 (tvar b x) T1 n1 ->
-      has_type GH G1 (tvar b x) T2 n2 ->
-      has_type GH G1 (tvar b x) (TAnd T1 T2) (S (n1+n2))
+  | T_AndI : forall GH G1 t T1 T2 n1 n2,
+      has_type GH G1 t T1 n1 ->
+      has_type GH G1 t T2 n2 ->
+      has_type GH G1 t (TAnd T1 T2) (S (n1+n2))
 
 (* : -- member initialization *)
 with dms_has_type: tenv -> venv -> dms -> ty -> nat -> Prop :=
